dist/gcc-compatible/Hacl_Hash_Blake2b_Simd256.c
@@ -556,22 +556,50 @@ static Hacl_Hash_Blake2b_Simd256_state_t
     (Lib_IntVector_Intrinsics_vec256 *)KRML_ALIGNED_MALLOC(32,
       sizeof (Lib_IntVector_Intrinsics_vec256) * 4U);
   memset(wv0, 0U, 4U * sizeof (Lib_IntVector_Intrinsics_vec256));
-  Lib_IntVector_Intrinsics_vec256
-  *b =
-    (Lib_IntVector_Intrinsics_vec256 *)KRML_ALIGNED_MALLOC(32,
-      sizeof (Lib_IntVector_Intrinsics_vec256) * 4U);
-  memset(b, 0U, 4U * sizeof (Lib_IntVector_Intrinsics_vec256));
   option___uint8_t___uint8_t___bool_____Lib_IntVector_Intrinsics_vec256_____Lib_IntVector_Intrinsics_vec256___
-  block_state =
+  block_state;
+  if (wv0 == NULL)
+  {
+    block_state =
+      (
+        (option___uint8_t___uint8_t___bool_____Lib_IntVector_Intrinsics_vec256_____Lib_IntVector_Intrinsics_vec256___){
+          .tag = FStar_Pervasives_Native_None
+        }
+      );
+  }
+  else
+  {
+    Lib_IntVector_Intrinsics_vec256
+    *b =
+      (Lib_IntVector_Intrinsics_vec256 *)KRML_ALIGNED_MALLOC(32,
+        sizeof (Lib_IntVector_Intrinsics_vec256) * 4U);
+    memset(b, 0U, 4U * sizeof (Lib_IntVector_Intrinsics_vec256));
+    if (b == NULL)
     {
-      .tag = FStar_Pervasives_Native_Some,
-      .v = {
-        .fst = kk.key_length,
-        .snd = kk.digest_length,
-        .thd = kk.last_node,
-        .f3 = { .fst = wv0, .snd = b }
-      }
-    };
+      KRML_ALIGNED_FREE(wv0);
+      block_state =
+        (
+          (option___uint8_t___uint8_t___bool_____Lib_IntVector_Intrinsics_vec256_____Lib_IntVector_Intrinsics_vec256___){
+            .tag = FStar_Pervasives_Native_None
+          }
+        );
+    }
+    else
+    {
+      block_state =
+        (
+          (option___uint8_t___uint8_t___bool_____Lib_IntVector_Intrinsics_vec256_____Lib_IntVector_Intrinsics_vec256___){
+            .tag = FStar_Pervasives_Native_Some,
+            .v = {
+              .fst = kk.key_length,
+              .snd = kk.digest_length,
+              .thd = kk.last_node,
+              .f3 = { .fst = wv0, .snd = b }
+            }
+          }
+        );
+    }
+  }
   if (block_state.tag == FStar_Pervasives_Native_None)
   {
     KRML_HOST_FREE(buf1);
@@ -610,10 +638,10 @@ static Hacl_Hash_Blake2b_Simd256_state_t
           p[0U] = s;
           if (p == NULL)
           {
-            Lib_IntVector_Intrinsics_vec256 *b0 = block_state1.f3.snd;
+            Lib_IntVector_Intrinsics_vec256 *b = block_state1.f3.snd;
             Lib_IntVector_Intrinsics_vec256 *wv = block_state1.f3.fst;
             KRML_ALIGNED_FREE(wv);
-            KRML_ALIGNED_FREE(b0);
+            KRML_ALIGNED_FREE(b);
             KRML_HOST_FREE(buf1);
             return NULL;
           }
@@ -1315,22 +1343,50 @@ Hacl_Hash_Blake2b_Simd256_state_t
     (Lib_IntVector_Intrinsics_vec256 *)KRML_ALIGNED_MALLOC(32,
       sizeof (Lib_IntVector_Intrinsics_vec256) * 4U);
   memset(wv0, 0U, 4U * sizeof (Lib_IntVector_Intrinsics_vec256));
-  Lib_IntVector_Intrinsics_vec256
-  *b =
-    (Lib_IntVector_Intrinsics_vec256 *)KRML_ALIGNED_MALLOC(32,
-      sizeof (Lib_IntVector_Intrinsics_vec256) * 4U);
-  memset(b, 0U, 4U * sizeof (Lib_IntVector_Intrinsics_vec256));
   option___uint8_t___uint8_t___bool_____Lib_IntVector_Intrinsics_vec256_____Lib_IntVector_Intrinsics_vec256___
-  block_state =
+  block_state;
+  if (wv0 == NULL)
+  {
+    block_state =
+      (
+        (option___uint8_t___uint8_t___bool_____Lib_IntVector_Intrinsics_vec256_____Lib_IntVector_Intrinsics_vec256___){
+          .tag = FStar_Pervasives_Native_None
+        }
+      );
+  }
+  else
+  {
+    Lib_IntVector_Intrinsics_vec256
+    *b =
+      (Lib_IntVector_Intrinsics_vec256 *)KRML_ALIGNED_MALLOC(32,
+        sizeof (Lib_IntVector_Intrinsics_vec256) * 4U);
+    memset(b, 0U, 4U * sizeof (Lib_IntVector_Intrinsics_vec256));
+    if (b == NULL)
     {
-      .tag = FStar_Pervasives_Native_Some,
-      .v = {
-        .fst = i.key_length,
-        .snd = i.digest_length,
-        .thd = i.last_node,
-        .f3 = { .fst = wv0, .snd = b }
-      }
-    };
+      KRML_ALIGNED_FREE(wv0);
+      block_state =
+        (
+          (option___uint8_t___uint8_t___bool_____Lib_IntVector_Intrinsics_vec256_____Lib_IntVector_Intrinsics_vec256___){
+            .tag = FStar_Pervasives_Native_None
+          }
+        );
+    }
+    else
+    {
+      block_state =
+        (
+          (option___uint8_t___uint8_t___bool_____Lib_IntVector_Intrinsics_vec256_____Lib_IntVector_Intrinsics_vec256___){
+            .tag = FStar_Pervasives_Native_Some,
+            .v = {
+              .fst = i.key_length,
+              .snd = i.digest_length,
+              .thd = i.last_node,
+              .f3 = { .fst = wv0, .snd = b }
+            }
+          }
+        );
+    }
+  }
   if (block_state.tag == FStar_Pervasives_Native_None)
   {
     KRML_HOST_FREE(buf);
@@ -1362,10 +1418,10 @@ Hacl_Hash_Blake2b_Simd256_state_t
           p[0U] = s;
           if (p == NULL)
           {
-            Lib_IntVector_Intrinsics_vec256 *b0 = block_state1.f3.snd;
+            Lib_IntVector_Intrinsics_vec256 *b = block_state1.f3.snd;
             Lib_IntVector_Intrinsics_vec256 *wv = block_state1.f3.fst;
             KRML_ALIGNED_FREE(wv);
-            KRML_ALIGNED_FREE(b0);
+            KRML_ALIGNED_FREE(b);
             KRML_HOST_FREE(buf);
             return NULL;
           }
